Adjustments to name visibility (of rmap, etc.) to better serve clients of the veric separation logic.

progs/verif1.v
@@ -1,5 +1,14 @@
 Require Import veric.base.
+Require Import veric.expr.
 Require Import veric.seplog.
+(* Require Import veric.SeparationLogic. 
+ Declare Module CSL: CLIGHT_SEPARATION_LOGIC. 
+  Import CSL. 
+*)
+
+Require veric.SequentialClight.
+Import SequentialClight.SeqC.CSL.
+
 Require Import veric.SequentialClight.
 Require Import msl.msl_standard.
 Require Import progs.list.
@@ -8,13 +17,13 @@ Module P := progs.test1.
 
 Import SeqC CSL.
 
-Definition sumlist_pre (contents: list int) (args: arguments) : predicate :=
+Definition sumlist_pre (contents: list int) (args: arguments) : pred rmap :=
   match args with 
   | p::nil => lseg (map (fun i => (Vint i, P.t_int)) contents) p (nullval, snd p)
   | _ => FF 
   end.
 
-Definition sumlist_post (contents: list int) (res: arguments) : predicate :=
+Definition sumlist_post (contents: list int) (res: arguments) : pred rmap :=
   match res with 
   | (Vint i, _) ::nil => prop (fold_right Int.add Int.zero contents = i)
   | _ => FF 
@@ -22,13 +31,13 @@ Definition sumlist_post (contents: list int) (res: arguments) : predicate :=
 
 Definition sumlist_fsig : funsig := (Tcons P.t_listptr Tnil, P.t_int).
 
-Definition reverse_pre (contents: list int) (args: arguments) : predicate :=
+Definition reverse_pre (contents: list int) (args: arguments) : pred rmap :=
   match args with 
   | p::nil => lseg (map (fun i => (Vint i, P.t_int)) contents) p (nullval, snd p)
   | _ => FF 
   end.
 
-Definition reverse_post (contents: list int) (res: arguments) : predicate :=
+Definition reverse_post (contents: list int) (res: arguments) : pred rmap :=
   match res with 
   | p::nil => lseg (map (fun i => (Vint i, P.t_int)) (rev contents)) p (nullval, snd p)
   | _ => FF 
@@ -45,6 +54,117 @@ Definition Gprog : funspecs :=
 nil.
 
 Ltac prove_notin := clear; simpl; intuition; match goal with H: _ = _ |- _ => inv H end.
+Definition bind_args' (formals: list (ident * type)) (P: arguments -> pred rmap) : assert :=
+   fun rho => P (map (fun xt => (eval_expr rho (Etempvar (fst xt) (snd xt)), snd xt)) formals).
+
+Lemma bind_args_eq: bind_args = bind_args'.
+Proof.
+intros.
+extensionality args P rho.
+unfold bind_args, bind_args'.
+f_equal.
+Qed.
+
+Lemma semax_post:
+ forall (R': ret_assert) Delta G (R: ret_assert) P c,
+   (forall ek vl rho, R' ek vl rho |-- R ek vl rho) ->
+   semax Delta G P c R' ->  semax Delta G P c R.
+Proof.
+intros; eapply semax_pre_post; eauto.
+Qed.
+
+Lemma semax_pre:
+ forall P' Delta G P c R,
+   (forall rho, P  rho |-- P' rho) ->   semax Delta G P' c R  -> semax Delta G P c R.
+Proof.
+intros; eapply semax_pre_post; eauto.
+Qed.
+
+Local Open Scope pred.
+
+
+Lemma env_gss:
+  forall rho id v t, eval_expr (env_set rho id v) (Etempvar id t) = v.
+Proof.
+intros.  unfold eval_expr, env_set; simpl. rewrite PTree.gss. simpl. auto.
+Qed.
+
+Lemma env_gso:
+  forall rho id id' v t, id <> id' -> 
+      eval_expr (env_set rho id' v) (Etempvar id t) = eval_expr rho (Etempvar id t).
+Proof.
+intros.  unfold eval_expr, env_set; simpl.
+rewrite PTree.gso by auto. auto.
+Qed.
+
+Definition force_int (v: val) := 
+ match v with
+ | Vint i => i | _ => Int.zero 
+ end.
+
+Definition sumlist_Inv (contents: list int) (rho: environ) : pred rmap :=
+          (Ex cts: list int, 
+           !!(fold_right Int.add Int.zero contents =
+             Int.add (force_int (eval_expr rho (Etempvar P.i_s P.t_int)))
+                       (fold_right Int.add Int.zero cts)) &&
+           lseg (map (fun i => (Vint i, P.t_int)) cts) 
+                 (eval_expr rho (Etempvar P.i_t P.t_listptr), P.t_listptr)
+                 (nullval, P.t_listptr)).
+
+Require Import veric.normalize.
+
+Lemma lseg_eq:
+  forall l v t, 
+  match t with Tpointer (Tstruct _ (Fcons _ _ (Fcons _ _ Fnil)) _) _ => True | _ => False end ->
+  typecheck_val v t = true ->
+    lseg l (v,t) (v,t) = !!(l=nil) && emp.
+Proof.
+intros.
+pose proof (lseg_unfold l (v,t) (v,t) (eq_refl _)).
+destruct t; try contradiction.
+destruct t; try contradiction.
+destruct f; try contradiction.
+destruct f; try contradiction.
+destruct f; try contradiction.
+simpl in *.
+destruct l.
+rewrite H1.
+f_equal.
+unfold ptr_eq.
+destruct v; simpl in H0; try discriminate.
+unfold Int.cmpu.
+rewrite Int.eq_true.
+normalize.
+replace (v0 :: l = nil) with False by (apply prop_ext; intuition; congruence).
+apply pred_ext; [ | normalize].
+rewrite H1; clear H1.
+normalize.
+destruct v; normalize.
+contradiction H1.
+simpl. split; auto. apply Int.eq_true.
+Qed.
+
+
+Lemma prop_right {A}{agA: ageable A}:
+  forall (P: pred A)(Q: Prop), Q -> (P |-- !!Q).
+Proof.
+intros; intros ? ?; auto.
+Qed.
+
+Lemma extract_exists_pre:
+      forall
+        (A : Type) (any: A) (P : A -> assert) (c : Clight.statement)
+         Delta (G : funspecs) (R : ret_assert),
+       (forall x : A, semax Delta G (P x) c R) ->
+       semax Delta G (fun rho => exp (fun x => P x rho)) c R.
+Proof.
+intros.
+apply semax_post with (existential_ret_assert (fun _:A => R)).
+intros ek vl rho w ?.
+simpl in H0. destruct H0; auto.
+apply extract_exists; auto.
+Qed.
+
 
 Lemma body_sumlist:
    semax_body Gprog P.f_sumlist _ sumlist_pre sumlist_post.
@@ -52,6 +172,100 @@ Proof.
 split; [split; simpl; repeat constructor; prove_notin | ].
 intro contents.
 simpl.
+unfold function_body_entry_assert, sumlist_pre.
+simpl fn_params.
+rewrite bind_args_eq.
+unfold bind_args'.
+simpl.
+set (contents' :=  map (fun i : int => (Vint i, P.t_int)) contents).
+unfold stackframe_of; simpl.
+apply semax_Sseq with
+  (fun rho => !! (eval_expr rho (Etempvar P.i_s P.t_int) = (Vint (Int.repr 0))) &&
+                              lseg contents' (eval_expr rho (Etempvar P.i_p P.t_listptr), P.t_listptr)
+                              (nullval, P.t_listptr)).
+evar (P1: assert); eapply semax_pre; [ | apply semax_set with (P:=P1)]; unfold P1; clear P1;
+   [ | | | reflexivity].
+intro. eapply derives_trans; [ |apply now_later].
+unfold subst.
+unfold overridePost. rewrite if_true by auto.
+apply prop_andp_right.
+rewrite env_gss. reflexivity.
+rewrite sepcon_emp.
+rewrite env_gso by (intro Hx; inv Hx); auto.
+admit.  (* typechecking proof *)
+reflexivity.
+apply semax_Sseq with
+  (fun rho => !! (eval_expr rho (Etempvar P.i_s P.t_int) = (Vint (Int.repr 0))
+                         /\ eval_expr rho (Etempvar P.i_t P.t_listptr) = eval_expr rho (Etempvar P.i_p P.t_listptr)) &&
+                              lseg contents' (eval_expr rho (Etempvar P.i_p P.t_listptr), P.t_listptr)
+                              (nullval, P.t_listptr)).
+evar (P1: assert); eapply semax_pre; [ | apply semax_set with (P:=P1)]; unfold P1; clear P1;
+   [ | | | reflexivity].
+intro. eapply derives_trans; [ |apply now_later].
+apply prop_andp_left; intro.
+unfold overridePost. rewrite if_true by auto.
+unfold subst.
+apply prop_andp_right.
+split.
+rewrite env_gso by (intro Hx; inv Hx); auto.
+rewrite env_gss. rewrite env_gso by (intro Hx; inv Hx); auto.
+rewrite env_gso by (intro Hx; inv Hx); auto.
+admit.  (* typechecking proof *)
+admit.  (* typechecking proof *)
+unfold contents'; clear contents'.
+ apply semax_pre with (sumlist_Inv contents).
+intro.
+apply prop_andp_left; intros [? ?].
+unfold sumlist_Inv.
+apply exp_right with contents.
+apply prop_andp_right.
+rewrite H. simpl.
+rewrite Int.add_zero_l. auto.
+rewrite H0. auto.
+apply semax_Sseq with
+  (fun rho => !!(fold_right Int.add Int.zero contents =
+              force_int (eval_expr rho (Etempvar P.i_s P.t_int)))).
+apply semax_while.
+admit.  (* typechecking proof *)
+reflexivity.
+intros.
+unfold assert_expr.
+apply prop_andp_left; intro.
+unfold Cnot in H.
+simpl in H.
+assert (eval_expr rho (Etempvar P.i_t P.t_listptr) = nullval).
+admit.
+unfold overridePost. rewrite if_true by auto.
+unfold sumlist_Inv.
+apply exp_left; intro cts.
+apply prop_andp_left; intro.
+rewrite H0.
+rewrite (lseg_eq (map (fun i : int => (Vint i, P.t_int)) cts) nullval P.t_listptr).
+2: simpl; auto.
+normalize.
+apply prop_right.
+rewrite H1. destruct cts; inv H2.  simpl fold_right. 
+rewrite Int.add_zero.  auto.
+admit.  (* typechecking proof *)
+unfold sumlist_Inv.
+apply semax_pre with 
+   (fun rho : environ =>
+    (Ex  cts : list int,
+   assert_expr (Etempvar P.i_t P.t_listptr) rho &&
+    !!(fold_right Int.add Int.zero contents =
+       Int.add (force_int (eval_expr rho (Etempvar P.i_s P.t_int)))
+         (fold_right Int.add Int.zero cts)) &&
+    lseg (map (fun i : int => (Vint i, P.t_int)) cts)
+      (eval_expr rho (Etempvar P.i_t P.t_listptr), P.t_listptr)
+      (nullval, P.t_listptr))).
+intro; normalize; intros.
+apply exp_right with x.
+repeat rewrite andp_assoc; auto.
+apply extract_exists_pre.
+apply nil.
+intro cts.
+
+
 
 Admitted.
 
